kuiops/sdpa/Kuiops.Sdpa.Flash.Barrier.fsti
@@ -192,16 +192,17 @@ fn barrier_ok
   (shQ : array2 et_ab (l2_row_major 16 (SZ.v d)))
   (eQsh : chest2 et_ab 16 (SZ.v d))
   (shM shL : array2 et_acc (l2_row_major (SZ.v nw) 16))
+  (eM eL : chest2 et_acc (SZ.v nw) 16)
   (shscale : array2 et_acc (l2_row_major (SZ.v nw) 16))
   (shO : array2 et_acc (l2_row_major (SZ.v nw * 16) (SZ.v d)))
   (shgl : array1 et_acc (l1_forward 16))
   (it : nat)
   requires
     forall+ (tid : natlt (block_threads nw)).
-      barrier_rin nw d shQ eQsh shM shL shscale shO shgl it tid
+      barrier_rin nw d shQ eQsh shM shL eM eL shscale shO shgl it tid
   ensures
     forall+ (tid : natlt (block_threads nw)).
-      barrier_rout nw d shQ eQsh shM shL shscale shO shgl it tid
+      barrier_rout nw d shQ eQsh shM shL eM eL shscale shO shgl it tid
 
 ghost
 fn flash_ml_to_pre
