kuiops/sdpa/Kuiops.Sdpa.Flash.fst
@@ -107,13 +107,19 @@ let sdpa_flash_kd
     let v = flash_views_of nw d sh in
     barrier_contract nw d v.shQv
       (flash_eQsh d b hq hkv group sq rows tiles eQ _bid)
-      v.shMv v.shLv v.shscalev v.shOv v.shglv);
+      v.shMv v.shLv
+      (flash_eM nw d b hq hkv group sq rows tiles sk eQ eK emask has_mask causal scale _bid)
+      (flash_eL nw d b hq hkv group sq rows tiles sk eQ eK emask has_mask causal scale _bid)
+      v.shscalev v.shOv v.shglv);
   barrier_count = (fun _ -> 3);
   barrier_ok = (fun _bid sh ->
     let v = flash_views_of nw d sh in
     FB.barrier_ok nw d v.shQv
       (flash_eQsh d b hq hkv group sq rows tiles eQ _bid)
-      v.shMv v.shLv v.shscalev v.shOv v.shglv);
+      v.shMv v.shLv
+      (flash_eM nw d b hq hkv group sq rows tiles sk eQ eK emask has_mask causal scale _bid)
+      (flash_eL nw d b hq hkv group sq rows tiles sk eQ eK emask has_mask causal scale _bid)
+      v.shscalev v.shOv v.shglv);
   frame = emp;
   block_pre = (fun bid ->
     flash_block_state nblk
